src/Util.v
@@ -550,3 +550,10 @@ Lemma zip_uniq_proj (T1 T2 : eqType) (s1 : seq T1) (s2 : seq T2) :
   by case: ifP=> [//| _]; apply (leq_trans IHl).
   Qed.
 
+  Lemma map_snd_zip_size (T U: Type) (s1 : seq T) (s2 : seq U) :
+    size s1 = size s2 -> map snd (zip s1 s2) = s2.
+  Proof.
+  elim: s2 s1=> [//|hd tl IHtl] [//|// a tla] eq_size /=.
+  by congr cons; rewrite IHtl //; move: eq_size=> /=[->].
+  Qed.
+
